

Option Pricing – Homework 6

Matheus Raka Pradnyatama

Problem 1.a)

At time T_2 :

The long position has a payoff: $S_{T_2} - K$

For the short position, we must pay: $-(S_{T_2} - F_t)$

Net payoff:

$$S_{T_2} - K - (S_{T_2} - F_t) = S_{T_2} - K - S_{T_2} + F_t = F_t - K$$

Therefore, accounting for the discount factor from time T_2 to t :

$$f_t = e^{-r*(T_2-t)} * (F_t - K)$$

Problem 1.b)

The strategy asks us to buy and hold the stock until time T_2 .

A stock, which is an agreement of ownership for a company, can be stored virtually in a virtual account (e.g. Robinhood account) or in a physical paper document until the future time T_2 , with no storage cost.

However, crude oil has some storage cost. We must have a sufficient physical space to store a barrel of crude oil and ensure that the storage has the right temperature and air exposure so that the oil doesn't go bad (as it is a chemical substance). Since there is some storage cost, F_t might not be enough to compensate us for all the expenses related to the storage cost and that the arbitrage strategy can fail in generating a profit.

Problem 1.e)

Isolating S_t term out from F_t

$$F_t = \exp \left\{ e^{-k*(T_2-t)} * \ln(S_t) + (1 - e^{-k*(T_2-t)})\alpha + \frac{\sigma^2}{4k} * (1 - e^{-2k*(T_2-t)}) \right\}$$

$$F_t = \exp \{ e^{-k*(T_2-t)} * \ln(S_t) \} * \exp \left\{ (1 - e^{-k*(T_2-t)})\alpha + \frac{\sigma^2}{4k} * (1 - e^{-2k*(T_2-t)}) \right\}$$

$$F_t = S_t^{e^{-k*(T_2-t)}} * \exp \left\{ (1 - e^{-k*(T_2-t)})\alpha + \frac{\sigma^2}{4k} * (1 - e^{-2k*(T_2-t)}) \right\}$$

$$f_t = e^{-r*(T_2-t)} * (S_{T_2} - F_t)$$

$$f_t = e^{-r*(T_2-t)} * \left(S_{T_2} - S_t^{e^{-k*(T_2-t)}} * \exp \left\{ (1 - e^{-k*(T_2-t)})\alpha + \frac{\sigma^2}{4k} * (1 - e^{-2k*(T_2-t)}) \right\} \right)$$

For $t = 0$,

$$f_0 = e^{-r*T_2} * \left(S_{T_2} - S_0^{e^{-k*T_2}} * \exp \left\{ (1 - e^{-k*T_2})\alpha + \frac{\sigma^2}{4k} * (1 - e^{-2k*T_2}) \right\} \right)$$

$$\frac{df_0}{dS} = e^{-r*T_2} * \left(1 - (e^{-k*T_2}) * S_0^{(e^{-k*T_2})-1} * \exp \left\{ (1 - e^{-k*T_2})\alpha + \frac{\sigma^2}{4k} * (1 - e^{-2k*T_2}) \right\} \right)$$

Exact solution is computed in the Jupyter Notebook.

Problem 1.f)

We have a short position for one call option. We want to hedge this.

Say we have a long position for n forward contracts.

Sensitivity of the long position should match the sensitivity of the short position.

$$n * \text{Forward Sensitivity} = \text{Call Sensitivity}$$

$$n * \frac{\partial f_0}{\partial S} = \frac{\partial C}{\partial S} = \Delta$$

$$n = \frac{\Delta}{\frac{\partial f_0}{\partial S}}$$

$$\text{Hedge Ratio} = \frac{\Delta}{\frac{\partial f_0}{\partial S}}$$

Exact solution is computed in the Jupyter Notebook.

Problem 1.g)

F_t is the time- t forward price for T_2 -delivery

At time- T_2 :

- The holder will receive delivery of θ barrel of crude oil, each with price S_{T_2}
- The holder will pay delivery price of K
- Payoff: $\theta * (S_{T_2} - K)$

At time- T_1 :

- The holder will see the forward price: F_{T_1} , for T_2 -delivery
- If the forward price is bigger than the delivery price, the holder will want to lock in the delivery price. He will want to buy more at the cheaper delivery price:
 - If $F_{T_1} > K$, then $\theta = 5,000$
- If the forward price is cheaper than the delivery price, the holder will want to buy less at the expensive delivery price:
 - If $F_{T_1} < K$, then $\theta = 4,000$

Computing the Time-0 Value

$$E[S_{T_2} | \mathcal{F}_{T_1}] = F_{T_1}$$

$$E[S_{T_2} - K | \mathcal{F}_{T_1}] = F_{T_1} - K$$

$$\theta * E[S_{T_2} - K | \mathcal{F}_{T_1}] = \theta * (F_{T_1} - K)$$

Using the discount factor, the time-0 value of the contract will be:

$$V_0 = E[e^{-rT_1} * \theta * (F_{T_1} - K)]$$

Use the mean to get the expected time-0 value of the payoff

Problem 2. a)

If S_t is a stock that continuously pays a constant proportional dividend yield q ,

The time- t forward price for time- T delivery of S_T is:

$$F_t = S_t * e^{(r-q)*(T-t)}$$

Therefore, **the time-0 forward price** for time- T delivery of S_T ,

$$F_0 = S_0 e^{(r-q)T}$$

Time-0 Value of Forward Contract, f_0

$$f_0 = e^{-rT} (F_0 - K)$$

$$f_0 = e^{-rT} (S_0 e^{(r-q)T} - K)$$

Using replication:

For the stock:

1 share of stock at time-0 $\rightarrow e^{qt}$ share of stock at time- t

a share of stock at time-0 $\rightarrow a * e^{qt}$ share of stock at time- t

For the bank account:

b unit of Bank at time-0 $\rightarrow b$ unit of Bank at time- t

$$\begin{aligned} V_t &= a * e^{qt} * S_t + b * B_t \\ V_t &= a * e^{qt} * S_t + b * e^{rt} \\ V_T &= a * e^{qT} * S_T + b * e^{rT} \end{aligned}$$

We want to replicate: $S_T - K$

$$\begin{aligned} V_T &= S_T - K \\ a * e^{qT} * S_T + b * e^{rT} &= S_T - K \end{aligned}$$

$$\begin{aligned} a * e^{qT} * S_T &= S_T \\ a * e^{qT} &= 1 \\ a &= e^{-qT} \end{aligned}$$

$$b * e^{rT} = -K$$

$$\begin{aligned} b &= -\frac{K}{e^{rT}} \\ b &= -K * e^{-rT} \end{aligned}$$

At time-0, the replicating portfolio holds:

e^{-qT} shares of S and $(-K e^{-rT})$ units of B .

Problem 2. b) At time T_0 , from the dividend payment, we will get:

$$x * D$$

We will then allocate the dividend into the bank account, so we need to multiply it with B_t .

At time t , the value of the replicating portfolio is:

$$V_t = x * S_t + (y + x * D * e^{-rT_0}) * B_t$$

$y * B_t$ is the original bank account balance

Now with an additional $x * D * e^{-rT_0} * B_t$ from the dividend

$$\begin{aligned} V_t &= x * S_t + (y + x * D * e^{-rT_0}) * e^{rt} \\ V_T &= x * S_T + (x * D * e^{r(T-T_0)}) + y * e^{rT} \end{aligned}$$

Set the replicating portfolio to $(S_T - K)$:

$$\begin{aligned} V_T &= S_T - K \\ x * S_T + (x * D * e^{r(T-T_0)}) + y * e^{rT} &= S_T - K \end{aligned}$$

$$\begin{aligned} x * S_T &= S_T \\ x &= 1 \end{aligned}$$

$$\begin{aligned} (x * D * e^{r(T-T_0)}) + y * e^{rT} &= -K \\ D e^{r(T-T_0)} + y * e^{rT} &= -K \\ y * e^{rT} &= -K - D e^{r(T-T_0)} \\ y &= -K * e^{-rT} - D e^{r(T-T_0)} e^{-rT} \\ y &= -K e^{-rT} - D e^{-rT_0} \end{aligned}$$

At time-0, the replicating portfolio holds:

1 share of S

$(-K e^{-rT} - D e^{-rT_0})$ units of B

Time-0 Value of Forward Contract, f_0

$$f_0 = x * S_0 + y * B_0 = x * S_0 + y * e^{r*0} = x * S_0 + y$$

$$f_0 = S_0 - K e^{-rT} - D e^{-rT_0}$$

Setting $f_0 = 0$,

$$\begin{aligned} S_0 - K * e^{-rT} - D e^{-rT_0} &= 0 \\ S_0 - D e^{-rT_0} &= K * e^{-rT} \\ K * e^{-rT} &= S_0 - D e^{-rT_0} \\ K &= e^{rT} (S_0 - D e^{-rT_0}) \end{aligned}$$

Time- 0 Forward Price, F_0

$$F_0 = K = e^{rT} (S_0 - D e^{-rT_0})$$

$$F_0 = e^{rT} (S_0 - D e^{-rT_0})$$